Update CounterRA

src/FairRA.v
@@ -1474,15 +1474,21 @@ Proof.
 Qed.
 
 Module ObligationRA.
-  Definition t: URA.t := @FiniteMap.t (@CounterRA.t Ord.t _).
+  Definition t: URA.t := @FiniteMap.t (URA.prod (@CounterRA.t Ord.t _) (OneShot.t unit)).
   Section RA.
     Context `{@GRA.inG t Σ}.
 
     Definition black (k: nat) (o: Ord.t): iProp :=
-      OwnM (FiniteMap.singleton k (CounterRA.black o: @CounterRA.t Ord.t _)).
+      OwnM (FiniteMap.singleton k ((CounterRA.black o: @CounterRA.t Ord.t _, ε: OneShot.t unit): URA.prod (@CounterRA.t Ord.t _) (OneShot.t unit))).
 
     Definition white (k: nat) (o: Ord.t): iProp :=
-      OwnM (FiniteMap.singleton k (CounterRA.white o: @CounterRA.t Ord.t _)).
+      OwnM (FiniteMap.singleton k ((CounterRA.white o: @CounterRA.t Ord.t _, ε: OneShot.t unit): URA.prod (@CounterRA.t Ord.t _) (OneShot.t unit))).
+
+    Definition pending (k: nat): iProp :=
+      OwnM (FiniteMap.singleton k ((ε: @CounterRA.t Ord.t _, OneShot.pending unit: OneShot.t unit): URA.prod (@CounterRA.t Ord.t _) (OneShot.t unit))).
+
+    Definition shot (k: nat): iProp :=
+      OwnM (FiniteMap.singleton k ((ε: @CounterRA.t Ord.t _, OneShot.shot tt: OneShot.t unit): URA.prod (@CounterRA.t Ord.t _) (OneShot.t unit))).
 
     Definition white_one k: iProp :=
       white k (Ord.S Ord.O).
@@ -1503,20 +1509,79 @@ Module ObligationRA.
       i. iIntros "POS". iPoseProof (black_persistent with "POS") as "POS". auto.
     Qed.
 
+    Lemma shot_persistent k
+      :
+      shot k -∗ □ shot k.
+    Proof.
+      iIntros "H".
+      unfold black.
+      iPoseProof (own_persistent with "H") as "H".
+      rewrite FiniteMap.singleton_core. auto.
+    Qed.
+
+    Global Program Instance Persistent_shot k: Persistent (shot k).
+    Next Obligation.
+    Proof.
+      i. iIntros "POS". ss. iPoseProof (shot_persistent with "POS") as "POS". auto.
+    Qed.
+
+    Lemma pending_unique k
+      :
+      (pending k)
+        -∗
+        (pending k)
+        -∗
+        False.
+    Proof.
+      iIntros "H0 H1". iCombine "H0 H1" as "H".
+      iOwnWf "H". rewrite FiniteMap.singleton_add in H0.
+      rewrite FiniteMap.singleton_wf in H0.
+      ur in H0. des. exfalso. eapply OneShot.pending_unique; eauto.
+    Qed.
+
+    Lemma pending_not_shot k
+      :
+      (pending k)
+        -∗
+        (shot k)
+        -∗
+        False.
+    Proof.
+      iIntros "H0 H1". iCombine "H0 H1" as "H".
+      iOwnWf "H". rewrite FiniteMap.singleton_add in H0.
+      rewrite FiniteMap.singleton_wf in H0.
+      ur in H0. des. exfalso. eapply OneShot.pending_not_shot; eauto.
+    Qed.
+
+    Lemma pending_shot k
+      :
+      (pending k)
+        -∗
+        #=> (shot k).
+    Proof.
+      iApply OwnM_Upd. eapply FiniteMap.singleton_updatable.
+      apply URA.prod_updatable.
+      { reflexivity. }
+      { apply OneShot.pending_shot. }
+    Qed.
+
     Lemma alloc o
       :
-      ⊢ #=> (∃ k, □ black k o ** white k o).
+      ⊢ #=> (∃ k, black k o ** white k o ** pending k).
     Proof.
       iPoseProof (@OwnM_unit _ _ H) as "H".
       iPoseProof (OwnM_Upd_set with "H") as "> H0".
       { eapply FiniteMap.singleton_alloc.
-        eapply CounterRA.black_white_wf.
+        instantiate (1:=((CounterRA.black o, ε): URA.prod (@CounterRA.t Ord.t _) (OneShot.t unit)) ⋅ ((CounterRA.white o, ε): URA.prod (@CounterRA.t Ord.t _) (OneShot.t unit)) ⋅ (ε, OneShot.pending unit)).
+        repeat rewrite unfold_prod_add. repeat rewrite URA.unit_idl. repeat rewrite URA.unit_id.
+        rewrite unfold_prod_wf. ss. split.
+        { eapply CounterRA.black_white_wf. }
+        { apply OneShot.pending_wf. }
       }
       iDestruct "H0" as "[% [% H0]]".
-      des. subst. erewrite <- FiniteMap.singleton_add.
-      iDestruct "H0" as "[H0 H1]".
+      des. subst. erewrite <- FiniteMap.singleton_add. erewrite <- FiniteMap.singleton_add.
+      iDestruct "H0" as "[[H0 H1] H2]".
       iModIntro. iExists _. iFrame.
-      iApply black_persistent. auto.
     Qed.
 
     Lemma black_mon o1 k o0
@@ -1525,6 +1590,7 @@ Module ObligationRA.
       black k o0 -∗ black k o1.
     Proof.
       iApply OwnM_extends. apply FiniteMap.singleton_extends.
+      apply URA.prod_extends. split; [|reflexivity].
       apply CounterRA.black_mon. auto.
     Qed.
 
@@ -1534,6 +1600,7 @@ Module ObligationRA.
       white k o1 -∗ #=> white k o0.
     Proof.
       iApply OwnM_Upd. apply FiniteMap.singleton_updatable.
+      apply URA.prod_updatable; [|reflexivity].
       apply CounterRA.white_mon. auto.
     Qed.
 
@@ -1556,7 +1623,9 @@ Module ObligationRA.
       iIntros "H0 H1". unfold white.
       replace (CounterRA.white (Hessenberg.add o0 o1): @CounterRA.t Ord.t ord_OrderedCM) with
         ((CounterRA.white o0: @CounterRA.t Ord.t _) ⋅ (CounterRA.white o1: @CounterRA.t Ord.t _)).
-      { iCombine "H0 H1" as "H". rewrite <- FiniteMap.singleton_add. iFrame. }
+      { iCombine "H0 H1" as "H". rewrite FiniteMap.singleton_add.
+        rewrite unfold_prod_add. rewrite URA.unit_id. auto.
+      }
       { symmetry. eapply (@CounterRA.white_split Ord.t ord_OrderedCM o0 o1). }
     Qed.
 
@@ -1567,10 +1636,12 @@ Module ObligationRA.
         (white k o0 ** white k o1).
     Proof.
       iIntros "H". unfold white.
-      replace (CounterRA.white (Hessenberg.add o0 o1): @CounterRA.t Ord.t ord_OrderedCM) with
-        ((CounterRA.white o0: @CounterRA.t Ord.t _) ⋅ (CounterRA.white o1: @CounterRA.t Ord.t _)).
+      replace (CounterRA.white (Hessenberg.add o0 o1): @CounterRA.t Ord.t ord_OrderedCM, ε: @OneShot.t unit) with
+        (((CounterRA.white o0, ε): URA.prod (@CounterRA.t Ord.t _) (OneShot.t unit)) ⋅ ((CounterRA.white o1, ε): URA.prod (@CounterRA.t Ord.t _) (OneShot.t unit))).
       { rewrite <- FiniteMap.singleton_add. iDestruct "H" as "[H0 H1]". iFrame. }
-      { symmetry. eapply (@CounterRA.white_split Ord.t ord_OrderedCM o0 o1). }
+      { rewrite unfold_prod_add. rewrite URA.unit_id. f_equal.
+        symmetry. eapply (@CounterRA.white_split Ord.t ord_OrderedCM o0 o1).
+      }
     Qed.
 
     Lemma white_split o0 o1 k o
@@ -1608,6 +1679,8 @@ Module ObligationRA.
       iCombine "H0 H1" as "H". rewrite FiniteMap.singleton_add.
       iOwnWf "H". iPureIntro.
       apply FiniteMap.singleton_wf in H0.
+      rewrite ! unfold_prod_add in H0.
+      rewrite unfold_prod_wf in H0. des. ss.
       apply CounterRA.black_white_compare in H0. auto.
     Qed.
 
@@ -1623,9 +1696,12 @@ Module ObligationRA.
       iCombine "H0 H1" as "H". rewrite FiniteMap.singleton_add.
       iPoseProof (OwnM_Upd_set with "H") as "> [% [% H]]".
       { eapply FiniteMap.singleton_updatable_set.
-        eapply CounterRA.black_white_decr.
+        rewrite unfold_prod_add. eapply URA.prod_updatable_set.
+        { eapply CounterRA.black_white_decr. }
+        { instantiate (1:=eq (ε ⋅ ε: OneShot.t unit)). ii. esplits; eauto. }
       }
-      { ss. des. subst. iModIntro. iExists _. iFrame. eauto. }
+      { ss. des. destruct m1. des; subst.
+        rewrite URA.unit_id. iModIntro. iExists _. iFrame. eauto. }
     Qed.
 
     Lemma black_white_decr_one k o1
